DeepFlow.v
@@ -1,0 +1,484 @@
+From Coq Require Import ZArith Lia Bool List String Program.Equality.
+From CDF Require Import Common Sequences Tactics Heaps HeapTactics.
+(* From CDF Require Import Separation2. *)
+From CDF Require Import DeepSeparation.
+(* From Coq Require Import ssreflect ssrfun ssrbool. *)
+
+Local Open Scope string_scope.
+(* Local Open Scope nat_scope. *)
+Local Open Scope Z_scope.
+Local Open Scope list_scope.
+
+Theorem ident_neq_sym : forall (n:ident) m, n <> m -> m <> n.
+Proof.
+  intros n m H1 H2; symmetry in H2; false_hyp H2 H1.
+Qed.
+
+(* Definition assertion := assertion val.
+Definition precond := assertion.
+Definition postcond := val -> assertion. *)
+
+Inductive expr : Type :=
+  | pvar (x: ident)
+  | pint (n: Z)
+  | plamb (x: ident) (n: expr)
+  | plet (x: ident) (e1: expr) (e2: expr)
+  (* | pref (x: ident) *)
+  (* | pderef (x: ident) *)
+  (* | passign (x1: ident) (x2: ident) *)
+  (* | pif (x: ident) (e1: expr) (e2: expr) *)
+  | pcall (x: ident) (a: ident)
+
+with val : Type :=
+  | vloc (i:Z)
+  | vint (i:Z)
+  (* need to relate free variables used in a lambda formula to those in the captured env *)
+  (* | vclos (x:ident) (e:expr) (s:store val) *)
+  | vclos (x:ident) (e:expr)
+
+with flow : Type :=
+  | req : sl val -> flow
+  | ens : option ident -> sl val -> flow
+  | seq : flow -> flow -> flow
+  | fexists : ident -> flow -> flow.
+
+Scheme expr_mut := Induction for expr Sort Prop
+with val_mut := Induction for val Sort Prop
+with flow_mut := Induction for flow Sort Prop.
+
+Coercion pint : Z >-> expr.
+Coercion vint : Z >-> val.
+
+Inductive eresult : Type :=
+  | enorm : val -> eresult.
+
+Reserved Notation " 'eval[' s ',' h ',' e ']' '=>' '[' s1 ',' h1 ',' r ']' " (at level 50, left associativity).
+
+Definition store := store val.
+Definition heap := heap val.
+
+Inductive bigstep : store -> heap -> expr -> store -> heap -> eresult -> Prop :=
+
+  | eval_pvar : forall s h x v,
+    Some v = s x ->
+    eval[ s, h, pvar x ]=>[ s, h, enorm v ]
+
+  | eval_plamb : forall s h x e,
+    eval[ s, h, plamb x e ]=>[ s, h, enorm (vclos x e) ]
+    (* eval[ s, h, plamb x e ]=>[ s, h, enorm (vclos x e s) ] *)
+
+  | eval_pint : forall s h x,
+    eval[ s, h, pint x ] => [ s, h, enorm (vint x) ]
+
+  | eval_plet : forall x e1 e2 v s h h2 s2 s1 h1 r,
+    eval[ s, h, e1 ] => [ s1, h1, enorm v] ->
+    eval[ supdate x v s1, h1, e2 ] => [ s2, h2, r] ->
+    eval[ s, h, plet x e1 e2 ] => [ s2, h2, r ]
+
+  | eval_pcall : forall fn x y e1 sf s h s2 h1 r arg,
+    (* s fn = Some (vclos y e1 sf) -> *)
+    s fn = Some (vclos y e1) ->
+    s x = Some arg ->
+    eval[ supdate y arg sf, h, e1 ] => [ s2, h1, r ] ->
+    eval[ s, h, pcall fn x ] => [ s, h1, r ]
+
+  (* | eval_pref : forall x s (h:heap) l,
+    h l = None ->
+    eval[ s, h, pref x ] => [ s, hupdate l (s x) h, enorm l]
+  | eval_deref : forall x s (h:heap) v,
+    h (s x) = Some v ->
+    eval[ s, h, pderef x ] => [ s, h, enorm v]
+  | eval_assign : forall x1 x2 s h,
+    eval[ s, h, passign x1 x2 ] => [ s, hupdate (s x1) (s x2) h, enorm 0] *)
+
+  where " 'eval[' s ',' h ',' e ']' '=>' '[' s1 ',' h1 ',' r ']' " := (bigstep s h e s1 h1 r).
+
+Module ProgramExamples.
+
+  (* Example ex_ref :
+    eval[ sempty, hempty, plet "x" (pconst 1) (pref "x") ]=>[ sempty, hupdate 2 1 hempty, enorm 2 ].
+  Proof.
+    apply eval_plet with (v:=1) (s1:=sempty) (s2:=supdate "x" 1 sempty) (h1:=hempty).
+    apply eval_pconst.
+    apply eval_pref.
+    constructor.
+  Qed. *)
+
+End ProgramExamples.
+
+
+(* Definition pts (x: ident) (y: ident) : assertion :=
+  fun s h =>
+    exists v w, Some (vint v) = s x /\ Some w = s y /\
+      (contains v w) s h.
+
+Definition ptsval (x: ident) (v: val) : assertion :=
+  fun s h =>
+    exists w, Some (vint w) = s x /\
+      (contains w v) s h. *)
+
+Inductive result : Type :=
+  | norm : val -> result.
+
+Definition compatible r1 r2 :=
+  match (r1, r2) with
+  | (norm r3, enorm r4) => r3 = r4
+end.
+
+(* Definition pure := pure val. *)
+
+Definition empty := ens None (pi (ptrue val)).
+
+Infix ";;" := seq (at level 80, right associativity).
+
+(* Fixpoint replace_val x v p := *)
+
+Fixpoint replace_ret (x:ident) (f:flow) :=
+  match f with
+  | ens (Some r) q => ens None (replace_sl r x q)
+  | ens None _ => f
+  | req _ => f
+  | a ;; b => a ;; (replace_ret x b)
+  | fexists i f => fexists i (replace_ret x f)
+  end.
+
+Definition compose (x:ident) (f1 f2:flow) : flow :=
+  fexists x (replace_ret x f1 ;; f2).
+
+Fixpoint fresh_in_flow (x:ident) (f:flow) :=
+  match f with
+  | ens (Some r) q => x <> r
+  | ens None q => True
+  | req _ => True
+  | seq a b => fresh_in_flow x a /\ fresh_in_flow x b
+  | fexists i f => x <> i /\ fresh_in_flow x f
+  end.
+
+Lemma fresh_replace : forall f x i,
+  fresh_in_flow i (replace_ret x f) ->
+  fresh_in_flow i f.
+Proof.
+  (* Check flow_mut. *)
+  apply (flow_mut (fun (e:expr) => True)
+    (fun (v:val) => True)
+    (fun (f0:flow) => forall (x i:ident),
+      fresh_in_flow i (replace_ret x f0) ->
+      fresh_in_flow i f0)); auto.
+  -
+  (* ens case, where there is now a binder *)
+  intros. destruct o; auto. unfold not; intros; subst. simpl in H. admit.
+  - simpl. intros. intuition auto.
+  apply H0 with (x:=x).
+  auto.
+  - simpl. intros.
+  intuition auto.
+  apply H with (x:=x).
+  intuition auto.
+Admitted.
+
+(* Reserved Notation " 'sem[' t ',' s ',' h ']=>[' t1 ',' s1 ',' h1 ',' r ']' '|=' f " (at level 50, left associativity). *)
+
+(* axiomatization of semantics for staged formulae *)
+(* Inductive satisfies : store -> heap -> store -> heap -> result -> flow -> Prop :=
+
+  | sat_req p s1 h1 s2 h2 r h3
+    (Hsu: s1 = s2)
+    (* h3 is the piece taken out satisfying p *)
+    (Hex: h1 = hunion h2 h3)
+    (Hd: hdisjoint h2 h3)
+    (Hp: p s1 h3) :
+    satisfies s1 h1 s2 h2 (norm r) (req p)
+
+  | sat_ens q s1 h1 s2 h2 h3 (v:val)
+    (Hsu:s1 = s2)
+    (* forall v, r = norm v -> *)
+    (* (Hr: r = norm v) *)
+    (* h3 is the piece satisfying q that is addded to h1 *)
+    (Hh: h2 = hunion h1 h3)
+    (Hd: hdisjoint h1 h3)
+    (Hq: q v s1 h3) :
+    satisfies s1 h1 s2 h2 (norm v) (ens q)
+
+  | sat_seq f1 f2 s1 h1 s2 h2 r s3 h3 r1
+    (Hs1: satisfies s1 h1 s3 h3 r1 f1)
+    (Hs2: satisfies s3 h3 s2 h2 r f2) :
+    satisfies s1 h1 s2 h2 r (seq f1 f2)
+
+  | sat_ex
+    x f s1 h1 s2 h2 r
+    (Hnotin: s1 x = None)
+    (Hfresh: fresh_in_flow x f)
+    (Hex: exists v, satisfies (supdate x v s1) h1 s2 h2 r f) :
+    satisfies s1 h1 s2 h2 r (fexists x f).
+
+  (* where " 'sem[' t ',' s ',' h ']=>[' t1 ',' s1 ',' h1 ',' r ']' '|=' f " := (satisfies t s h t1 s1 h1 r f) *)
+
+(** Result can be anything if unconstrained *)
+Lemma unconstrained_res : forall s h v,
+  satisfies s h s h (norm v) empty.
+Proof.
+  intros.
+  apply sat_ens with (h3:=hempty); heap.
+  unfold pure.
+  auto.
+Qed.
+
+(** replace_ret removes the result value and constrains the given variable *)
+Example e_replace_ret : forall x s h,
+  satisfies s h s h (norm 2) (replace_ret x (ens (fun r => pure (r = 1)))) <->
+    satisfies s h s h (norm 2) (ens (fun r s h => s x = Some (vint 1))).
+Proof.
+  split.
+  - intros.
+    simpl in H.
+    inv H.
+    destr_all.
+    unfold pure in H2.
+    destr H2.
+    subst.
+    apply sat_ens with (h3:=hempty); auto.
+  - intros.
+    simpl.
+    inv H.
+    apply sat_ens with (h3:=hempty); heap.
+    exists 1.
+    intuition easy.
+Qed.
+
+Module SemanticsExamples.
+
+  (* ex z; req x->z; ens[r] x->1/\r=1 *)
+  Definition f3 : flow :=
+    fexists "z" (req (pts "x" "z") ;; ens (fun r => (r = 1) //\\ ptsval "x" 1)).
+
+  Example ex_sem_f3:
+    satisfies (supdate "x" (vint 2) sempty) (hupdate 2 (vint 3) hempty)
+      (supdate "z" (vint 3) (supdate "x" (vint 2) sempty)) (hupdate 2 (vint 1) hempty) (norm (vint 1)) f3.
+  Proof.
+    unfold f3.
+    apply sat_ex.
+    heap.
+    easy.
+    exists (vint 3).
+    apply sat_seq with (s3:=supdate "z" (vint 3) (supdate "x" (vint 2) sempty)) (h3:=hempty) (r1:=norm (vint 5)).
+    - apply sat_req with (h3:=hupdate 2 (vint 3) hempty).
+      reflexivity.
+      heap.
+      heap.
+      unfold pts.
+      exists 2.
+      exists (vint 3).
+      intuition easy.
+    - apply sat_ens with (h3:=hupdate 2 (vint 1) hempty); heap.
+      (* rewrite supdate_dupe. *)
+      (* reflexivity. *)
+      unfold pureconj.
+      unfold ptsval.
+      intuition.
+      exists 2.
+      intuition.
+      unfold contains.
+      heap.
+  Qed.
+
+End SemanticsExamples.
+
+
+(* forward rules say how to produce a staged formula from a program *)
+Inductive forward : expr -> flow -> Prop :=
+  | fw_int: forall i p,
+    p = (ens (fun res => (res = vint i) //\\ emp)) ->
+    forward (pint i) p
+
+  | fw_lamb: forall x p e,
+    (* cannot check the spec at this point, as lambdas containing flows would be mutually recursive *)
+    (* p = (ens (fun res => (res = vclos x e s) //\\ emp)) -> *)
+    p = (ens (fun res => (res = vclos x e) //\\ emp)) ->
+    forward (plamb x e) p
+
+  | fw_var: forall x p,
+    p = (ens (fun res s h => exists v, s x = Some v /\ res = v /\ emp s h)) ->
+    forward (pvar x) p
+
+  (* | fw_deref: forall x y,
+    forward (pderef x) (fexists y (req (pts x y);;
+      ens (fun res s h => ((res = s y) //\\ pts x y) s h)))
+
+  | fw_ref: forall x y,
+    (* forward (pref x) (fexists (fun y => ens (fun r s h => contains y (s x) s h))) *)
+    forward (pref x) (fexists y (ens (fun r s h => (r = s y) /\ (pts y x s h)))) *)
+
+  | fw_let: forall x e1 e2 f1 f2,
+    forward e1 f1 ->
+    forward e2 f2 ->
+    (* replace_ret x f1 = f3 -> *)
+    (* f1 ;; ens (fun _ => ) = f3 -> *)
+    (* forward (plet x e1 e2) (fexists x (f3 ;; f2)) *)
+    forward (plet x e1 e2) (compose x f1 f2)
+
+  (* | fw_get: forall l v, 
+    forward (GET l)
+      (req (contains l v) ;;
+      (ens (fun r => (r = v) //\\ contains l v))) *)
+.
+
+Example e_fw_let : forall x,
+  forward (plet x 1 (pvar x)) (fexists x (
+    replace_ret x (ens (fun r => pure (r = 1))) ;;
+    ens (fun res s h => exists v, Some v = s x /\ res = v /\ emp s h)
+    )).
+Proof.
+  simpl.
+  intros.
+  apply fw_let with (f1 := (ens (fun r => pure (r = 1)))).
+  - eapply fw_int.
+    reflexivity.
+  - apply fw_var.
+    (* trivial from here, but we have to go through this whole song and dance *)
+    f_equal.
+    post_ext.
+    split; intros.
+    + destr H.
+      intuition.
+      exists H0.
+      intuition auto.
+    + destr H.
+      exists H0.
+      intuition auto.
+Qed.
+
+(** The semantics only grows the store. *)
+Definition satisfies_monotonic : forall f s1 h1 s2 h2 r,
+  satisfies s1 h1 s2 h2 r f -> substore s1 s2.
+Proof.
+  induction f; intros.
+  - inv H. ok.
+  - inv H. ok.
+  - inv H.
+    specialize (IHf1 _ _ _ _ _ Hs1).
+    specialize (IHf2 _ _ _ _ _ Hs2).
+    apply substore_trans with (s2 := s4); auto.
+  - inv H.
+    destruct Hex as [v Hsat].
+    specialize (IHf _ _ _ _ _ Hsat).
+    specialize (substore_reduce_left _ _ _ _ _ Hnotin IHf).
+    ok.
+Qed.
+
+Lemma satisfies_replace_ret : forall f x v s1 h1 s2 h2 r,
+  fresh_in_flow x f ->
+  s1 x = Some v ->
+  satisfies s1 h1 s2 h2 r (replace_ret x f) ->
+  satisfies s1 h1 s2 h2 (norm v) f.
+Proof.
+  induction f; intros; simpl in *.
+  - inv H1.
+    apply sat_req with (h3 := h4); ok.
+  - inv H1. destruct Hq as [v1 [H3 H2]].
+    rewrite H3 in H0; inj H0.
+    apply sat_ens with (h3 := h4); ok.
+  - inv H1.
+    pose proof (satisfies_monotonic _ _ _ _ _ _ Hs1) as Hmono1.
+    pose proof (substore_mem _ s1 s4 v x Hmono1 H0) as Hs.
+    destruct H as [Hf1 Hf2].
+    specialize (IHf2 x v s4 h4 s2 h2 r Hf2 Hs Hs2).
+    apply sat_seq with (s3:=s4) (h3:=h4) (r1:=r1); ok.
+  - inv H1; destruct Hex as [v0 Hsat].
+    destruct H as [Hneq Hf].
+    pose proof (ident_neq_sym _ _ Hneq) as Hneq1.
+    pose proof (supdate_other _ s1 i v0 x Hneq1) as He. rewrite <- He in H0.
+    specialize (IHf x v (supdate i v0 s1) h1 s2 h2 r Hf H0 Hsat).
+    apply sat_ex; auto.
+    apply fresh_replace with (x:=x); easy.
+    exists v0.
+    auto.
+Qed.
+
+Theorem soundness :
+  forall se1 he1 e se2 he2 re (**) f ss1 hs1 ss2 hs2 rs,
+    bigstep se1 he1 e se2 he2 re ->
+    substore se1 ss1 ->
+    (* he1 = hs1 -> *)
+    forward e f ->
+    satisfies ss1 hs1 ss2 hs2 rs f ->
+    substore se2 ss2
+    (* /\ he2 = hs2 *)
+    /\ compatible rs re.
+Proof.
+  intros se1 he1 e se2 he2 re
+          f ss1 hs1 ss2 hs2 rs
+          Hb.
+  revert f ss1 hs1 ss2 hs2 rs.
+  induction Hb;
+  intros f ss1 hs1 ss2 hs2 rs;
+  intros Hsub Hf Hs.
+  - (* var. the proof comes down to the fact that both spec and program read
+        s(x) and leave the heap unchanged. *)
+    inv Hf.
+    inv Hs.
+    destr_all; subst.
+    intuition.
+    unfold compatible.
+    unfold emp in H4.
+    subst.
+    unfold substore in Hsub.
+    symmetry in H.
+    specialize (Hsub v x H).
+    congruence.
+  - (* lambda case *)
+    inv Hf.
+    (* destruct H2 as [s0 Hq]. *)
+    (* subst. *)
+    inv Hs.
+    unfold pureconj in Hq.
+    unfold compatible.
+    intuition auto.
+  - (* int *)
+    inv Hf.
+    inv Hs.
+    unfold compatible.
+    unfold pureconj in Hq.
+    intuition auto.
+  - (* let *)
+    (* we have an IH for each subexpr *)
+    (* v is the intermediate result of evaluating e1 *)
+    (* r is the final result *)
+    inv Hf.
+    (* the spec is of the form ex x. f1[x/r];f2 *)
+    (* see how it evaluates *)
+    inv Hs.
+    destruct Hex as [v1 Hseq].
+    (* v1 is the return value of f1, which can be anything due to replace ret *)
+    inv Hseq.
+
+    (* reason about replace_ret using the freshness of existentials *)
+    pose proof (satisfies_replace_ret f1 x v1 (supdate x v1 ss1) hs1 s4 h4 r1) as Hrr.
+    forward Hrr. {
+      simpl in Hfresh.
+      destruct Hfresh as [Hfresh _].
+      apply (fresh_replace _ _ _ Hfresh).
+    }
+    forward Hrr by apply supdate_same.
+    specialize (Hrr Hs1).
+    clear Hfresh.
+
+    (* apply IH1 to know that all of e1 is sound *)
+    specialize (IHHb1 f1 (supdate x v1 ss1) hs1 s4 h4 (norm v1)).
+    forward IHHb1 by apply substore_extension_trans with (s2:=ss1); auto.
+    specialize (IHHb1 H3 Hrr).
+    destruct IHHb1 as [Hst Hcomp].
+    unfold compatible in Hcomp; subst.
+
+    (* apply IH2 to know that the entire thing is sound *)
+    specialize (IHHb2 f2 s4 h4 ss2 hs2 rs).
+    forward IHHb2. {
+      pose proof (satisfies_monotonic _ _ _ _ _ _ Hs1) as Hmono.
+      specialize (substore_extension_left _ s1 s4 v x Hst) as Hsub1.
+      now forward Hsub1 by apply (substore_extension_inv _ _ _ _ _ Hmono).
+    }
+    specialize (IHHb2 H4 Hs2).
+    easy.
+  - (* call *)
+  inv Hf.
+(* Qed. *)
+Admitted. *)
